Refactor everything to use bullets, better indentation, etc.

src/Searchability.v
@@ -1,43 +1,45 @@
 CoInductive conat : Type :=
 {
-    pred : option conat
+  pred : option conat;
 }.
 
 Class Searchable (A : Type) : Type :=
 {
-    search : (A -> bool) -> A;
-    search_spec :
-      forall p : A -> bool,
-        p (search p) = true \/
-        forall x : A, p x = false;
+  search : (A -> bool) -> A;
+  search_spec :
+    forall p : A -> bool,
+      p (search p) = true \/
+      forall x : A, p x = false;
 }.
 
 Definition zero : conat :=
 {|
-    pred := None
+  pred := None
 |}.
 
 Definition succ (c : conat) : conat :=
 {|
-    pred := Some c
+  pred := Some c
 |}.
 
 CoFixpoint omega : conat :=
 {|
-    pred := Some omega
+  pred := Some omega
 |}.
 
 CoFixpoint search_conat (p : conat -> bool) : conat :=
 {|
-    pred := if p zero
-            then None
-            else Some (search_conat (fun n => p (succ n)))
+  pred :=
+    if p zero
+    then None
+    else Some (search_conat (fun n => p (succ n)))
 |}.
 
 Lemma eq_pred :
-  forall n m : conat, pred n = pred m -> n = m.
+  forall n m : conat,
+    pred n = pred m -> n = m.
 Proof.
-  destruct n, m. cbn. destruct 1. reflexivity.
+  now intros [] []; cbn; intros ->.
 Qed.
 
 Lemma sc_eq :
@@ -45,39 +47,44 @@ Lemma sc_eq :
     search_conat p =
       if p zero then zero else succ (search_conat (fun n => p (succ n))).
 Proof.
-  intros. apply eq_pred. cbn.
-  destruct (p zero) eqn: Hp; cbn; reflexivity.
+  intros p.
+  apply eq_pred; cbn.
+  now destruct (p zero); cbn.
 Qed.
 
 CoInductive sim (n m : conat) : Prop :=
 {
-    sim' :
-      (pred n = None /\ pred m = None) \/
-      (exists n' m' : conat,
-        pred n = Some n' /\ pred m = Some m' /\ sim n' m')
+  sim' :
+    (pred n = None /\ pred m = None) \/
+    (exists n' m' : conat,
+      pred n = Some n' /\ pred m = Some m' /\ sim n' m')
 }.
 
 Lemma search_conat_spec :
   forall p : conat -> bool,
-    p (search_conat p) = false -> sim (search_conat p) omega.
+    p (search_conat p) = false ->
+      sim (search_conat p) omega.
 Proof.
   cofix CH.
-  intros p H.
-  constructor. cbn. destruct (p zero) eqn: Hp.
-  - replace (search_conat p) with zero in H.
-    + congruence.
-    + apply eq_pred. cbn. rewrite Hp. reflexivity.
-  - right. do 2 eexists. split; [| split].
-    1-2: reflexivity.
-    apply CH. rewrite sc_eq, Hp in H. assumption.
+  intros p Hf.
+  constructor; cbn.
+  destruct (p zero) eqn: Hp.
+  - replace (search_conat p) with zero in Hf; [now congruence |].
+    apply eq_pred; cbn.
+    now rewrite Hp.
+  - right.
+    do 2 eexists.
+    do 2 split; [easy |].
+    apply CH.
+    now rewrite sc_eq, Hp in Hf.
 Qed.
 
 CoInductive le (n m : conat) : Prop :=
 {
-    le' :
-      pred n = None \/
-      (exists n' m' : conat,
-        pred n = Some n' /\ pred m = Some m' /\ le n' m')
+  le' :
+    pred n = None \/
+    (exists n' m' : conat,
+      pred n = Some n' /\ pred m = Some m' /\ le n' m')
 }.
 
 Lemma sc_true :
@@ -85,56 +92,56 @@ Lemma sc_true :
     p n = true -> le (search_conat p) n.
 Proof.
   cofix CH.
-  intros p n H.
-  constructor. rewrite sc_eq. destruct (p zero) eqn: Hp.
-  - left. cbn. reflexivity.
-  - right. cbn. destruct n as [[n' |]].
-    + do 2 eexists; split; [| split].
-      1-2: reflexivity.
-      apply CH. unfold succ. assumption.
-    + unfold zero in Hp. congruence.
+  intros p n Ht.
+  constructor.
+  rewrite sc_eq.
+  destruct (p zero) eqn: Hp; cbn; [now left |].
+  right.
+  destruct n as [[n' |]]; [| now unfold zero in Hp; congruence].
+  do 2 eexists.
+  do 2 split; [easy |].
+  apply CH.
+  now unfold succ.
 Qed.
 
 Lemma le_omega_l :
-  forall n : conat, le omega n -> sim n omega.
+  forall n : conat,
+    le omega n -> sim n omega.
 Proof.
   cofix CH.
-  intros n H. destruct H as [[|]].
-  - cbn in H. inversion H.
-  - destruct H as (omega' & n' & H1 & H2 & H3).
-    cbn in *; inversion H1; subst; clear H1.
-    constructor. right. exists n', omega. cbn.
-    split; [| split].
-    + assumption.
-    + reflexivity.
-    + apply CH. assumption.
+  intros n [[| (omega' & n' & H1 & H2 & H3)]]; cbn in *; [easy |].
+  injection H1 as [= <-].
+  constructor; right.
+  exists n', omega.
+  split; [easy |].
+  split; [easy |].
+  now apply CH.
 Qed.
 
 Axiom sim_eq :
-  forall n m : conat, sim n m -> n = m.
+  forall n m : conat,
+    sim n m -> n = m.
 
 #[refine]
 Instance Searchable_conat : Searchable conat :=
 {
-    search := search_conat;
+  search := search_conat;
 }.
 Proof.
-  intro p. destruct (p (search_conat p)) eqn: H; [left; reflexivity |].
-  right. intro n.
-  destruct (p n) eqn: Hpn; [| reflexivity].
+  intros p.
+  destruct (p (search_conat p)) eqn: Hpscp; [now left |].
+  right; intros n.
+  destruct (p n) eqn: Hpn; [| easy].
   assert (Heq : search_conat p = omega).
   {
-    apply sim_eq.
-    apply search_conat_spec.
-    assumption.
+    now apply sim_eq, search_conat_spec.
   }
   assert (Heq' : n = omega).
   {
-    apply sim_eq.
-    apply le_omega_l.
+    apply sim_eq, le_omega_l.
     rewrite <- Heq.
-    apply sc_true.
-    assumption.
+    now apply sc_true.
   }
-  rewrite Heq in *; subst. congruence.
+  rewrite Heq in Hpscp; subst.
+  now congruence.
 Defined.
