src/ConaturalExercises.v
@@ -2,85 +2,88 @@
 
 (** ** The basics *)
 
-(** Conatural numbers are things that [option]ally can have a predecessor
-    which is a conatural number too. Contrast this with naturals, which
-    are either zero or a successor of a natural number - we see that [nat]
-    and [conat] are dual. *)
+(**
+  Conatural numbers are things that [option]ally can have a predecessor
+  which is a conatural number too. Contrast this with naturals, which
+  are either zero or a successor of a natural number - we see that [nat]
+  and [conat] are dual.
+*)
 
 CoInductive conat : Type :=
 {
-    pred : option conat;
+  pred : option conat;
 }.
 
-(** [sim] (an abbreviation of "bisimilarity") is our custom "equality" for
-    conatural numbers. The ordinary equality won't do, because it is not fit
-    for use with (possibly) infinite objects.
+(**
+  [sim] (an abbreviation of "bisimilarity") is our custom "equality" for
+  conatural numbers. The ordinary equality won't do, because it is not fit
+  for use with (possibly) infinite objects.
 
-    Two conaturals are bisimilar when either they are zero or they have bisimilar
-    predecessors. *)
+  Two conaturals are bisimilar when either they are zero or they have bisimilar
+  predecessors.
+*)
 
 CoInductive sim (n m : conat) : Prop :=
 {
-    sim' :
-      (pred n = None /\ pred m = None)
-        \/
-      (exists n' m' : conat,
-        pred n = Some n' /\ pred m = Some m' /\ sim n' m');
+  sim' :
+    (pred n = None /\ pred m = None)
+      \/
+    (exists n' m' : conat,
+      pred n = Some n' /\ pred m = Some m' /\ sim n' m');
 }.
 
-(** Using [sim] instead of [eq] saves us from trouble when proving, but it
-    doesn't save us from having to prove a lot of auxiliary lemmas... unless
-    we use the axiom [sim_eq], which says that bisimilar conaturals are equal.
+(**
+  Using [sim] instead of [eq] saves us from trouble when proving, but it
+  doesn't save us from having to prove a lot of auxiliary lemmas... unless
+  we use the axiom [sim_eq], which says that bisimilar conaturals are equal.
 
-    Feel free to use this axiom - it is consistent with Coq's logic - but
-    ideally you should avoid it. *)
+  Feel free to use this axiom - it is consistent with Coq's logic - but
+  ideally you should avoid it.
+*)
 
 Axiom sim_eq :
   forall {n m : conat}, (sim n m) = (n = m).
 
-(** [eq_pred] is a very useful lemma - conaturals with equal predecessors are
-    equal. To prove it, it suffices to [destruct] both [n] and [m] and then
-    [rewrite] the hypothesis. *)
+(**
+  [eq_pred] is a very useful lemma - conaturals with equal predecessors are
+  equal. To prove it, it suffices to [destruct] both [n] and [m] and then
+  [rewrite] the hypothesis.
+*)
 
 Lemma eq_pred :
   forall n m : conat, pred n = pred m -> n = m.
 Proof.
-  intros [] [] H.
-  cbn in H.
-  rewrite H.
-  reflexivity.
+  now intros [] []; cbn; intros ->.
 Qed.
 
-(** This tactic will prove very useful for you... *)
+(**
+  We prove theorems about conatural numbers (and about inhabitants of other
+  coinductive types) using the [cofix] tactic. It is a very primitive tactic,
+  dual to the [fix] tactic used for proofs by induction. Sadly, there just
+  isn't a better way.
 
-Ltac inv H := inversion H; subst; clear H; auto.
+  Let's try to prove that [sim] is reflexive, i.e. [forall n : conat, sim n n].
 
-(** We prove theorems about conatural numbers (and about inhabitants of other
-    coinductive types) using the [cofix] tactic. It is a very primitive tactic,
-    dual to the [fix] tactic used for proofs by induction. Sadly, there just
-    isn't a better way.
+  In our first proof attempt below, we start with [cofix CH], which introduces
+  the coinduction hypothesis [CH : forall n : conat, sim n n] to the context.
+  It looks like we are done, as we can use [CH] to finish the theorem, but this
+  is a deadly trap - the command [Admitted] would fail at this point. This is because
+  before we can use the coinduction hypothesis, we must produce a part of the
+  result (which here is just a step of the proof), similarly to how we can apply
+  the induction hypothesis only after we reduce the problem in size.
 
-    Let's try to prove that [sim] is reflexive, i.e. [forall n : conat, sim n n].
-
-    In our first proof attempt below, we start with [cofix CH], which introduces
-    the coinduction hypothesis [CH : forall n : conat, sim n n] to the context.
-    It looks like we are done, as we can use [CH] to finish the theorem, but this
-    is a deadly trap - the command [Admitted] would fail at this point. This is because
-    before we can use the coinduction hypothesis, we must produce a part of the
-    result (which here is just a step of the proof), similarly to how we can apply
-    the induction hypothesis only after we reduce the problem in size.
-
-    We start our second proof attempt in the same way, by giving ourselves the
-    coinduction hypothesis [CH : forall n : conat, sim n n]. This time, however,
-    we use the [constructor] tactic to make make a step towards proving [sim n n].
-    We have two possibilities: [n] is bisimilar to [n] either because both are
-    zero (i.e. have no predecessor) or because both have bisimilar predecessors.
-    To decide which case it is, we destruct [n], naming the predecessor [n'].
-    In the first case ([n] has predecessor [n']), we go right, tell Coq that the
-    predecessor is [n'], solve the trivial side goals, and finish the proof by
-    using the coinduction hypothesis to show that the predecessor is bisimilar
-    to itself (i.e. [sim n' n']). The second case ([n] has no predecessor) is
-    trivial. *)
+  We start our second proof attempt in the same way, by giving ourselves the
+  coinduction hypothesis [CH : forall n : conat, sim n n]. This time, however,
+  we use the [constructor] tactic to make make a step towards proving [sim n n].
+  We have two possibilities: [n] is bisimilar to [n] either because both are
+  zero (i.e. have no predecessor) or because both have bisimilar predecessors.
+  To decide which case it is, we destruct [n], naming the predecessor [n'].
+  In the first case ([n] has predecessor [n']), we go right, tell Coq that the
+  predecessor is [n'], solve the trivial side goals, and finish the proof by
+  using the coinduction hypothesis to show that the predecessor is bisimilar
+  to itself (i.e. [sim n' n']). The second case ([n] has no predecessor) is
+  trivial.
+*)
 
 Lemma sim_refl :
   forall n : conat, sim n n.
@@ -91,82 +94,95 @@ Proof.
 Restart.
   cofix CH.
   constructor.
-  destruct n as [[n' |]]; cbn.
-  - right. exists n', n'. split; [| split].
-    1-2: reflexivity.
-    apply CH.
-  - left. intuition.
+  destruct n as [[n' |]]; cbn; [| now left].
+  right.
+  exists n', n'.
+  split; [easy |].
+  split; [easy |].
+  now apply CH.
 Qed.
 
-(** Heads up, coinduction is easy! Now, try some proofs by coinduction to
-    see for yourself. *)
+(**
+  Heads up, coinduction is easy! Now, try some proofs by coinduction to
+  see for yourself.
+*)
 
 Lemma sim_sym :
-  forall n m : conat, sim n m -> sim m n.
+  forall n m : conat,
+    sim n m -> sim m n.
 Proof.
 Admitted.
 
 Lemma sim_trans :
-  forall a b c : conat, sim a b -> sim b c -> sim a c.
+  forall a b c : conat,
+    sim a b -> sim b c -> sim a c.
 Proof.
 Admitted.
 
-(** We import [Setoid] so that we can [rewrite] with [sim] the same way we can
-    rewrite with ordinary equality. *)
+(**
+  We import [Setoid] so that we can [rewrite] with [sim] the same way we can
+  rewrite with ordinary equality.
+*)
 
-Require Import Setoid.
+From Stdlib Require Import Setoid.
 
-Instance Equivalence_sim : Equivalence sim.
+#[export] Instance Equivalence_sim : Equivalence sim.
 Proof.
-  esplit; red.
-    apply sim_refl.
-    apply sim_sym.
-    apply sim_trans.
+  split; red.
+  - now apply sim_refl.
+  - now apply sim_sym.
+  - now apply sim_trans.
 Defined.
 
 (** ** Zero, successor and infinity *)
 
-(** We can now define some basic conatural numbers and functions. [zero] is
-    the conatural number that has no predecessor. The [succ]essor of [n] is
-    the conatural whose [pred]ecessor is [n]. *)
+(**
+  We can now define some basic conatural numbers and functions. [zero] is
+  the conatural number that has no predecessor. The [succ]essor of [n] is
+  the conatural whose [pred]ecessor is [n].
+*)
 
 Definition zero : conat :=
 {|
-    pred := None;
+  pred := None;
 |}.
 
 Definition succ (n : conat) : conat :=
 {|
-    pred := Some n;
+  pred := Some n;
 |}.
 
-(** But a much more interesting case is [omega], the infinite conatural number.
-    It is defined as the conatural number which is its own predecessor.
+(**
+  But a much more interesting case is [omega], the infinite conatural number.
+  It is defined as the conatural number which is its own predecessor.
 
-    To define infinite values of coinductive types (and functions into coinductive
-    types), we use the keyword [CoFixpoint]. Remember that, just like for proofs
-    by coinduction, we must produce a part of the object we're defining before we
-    can make any use of the corecursive call. For conaturals, this means that the
-    corecursive call must occur inside of [{| pred := ... |}]. *)
+  To define infinite values of coinductive types (and functions into coinductive
+  types), we use the keyword [CoFixpoint]. Remember that, just like for proofs
+  by coinduction, we must produce a part of the object we're defining before we
+  can make any use of the corecursive call. For conaturals, this means that the
+  corecursive call must occur inside of [{| pred := ... |}].
+*)
 
 CoFixpoint omega : conat :=
 {|
-    pred := Some omega;
+  pred := Some omega;
 |}.
 
-(** Congratulations on reaching the end of this short tutorial - I don't have
-    enough time for more explanations... in case of doubt, refer to
-    https://coq.inria.fr/refman/language/core/coinductive.html
-    to read a bit more about coinduction and to
-    https://coq.inria.fr/refman/proofs/writing-proofs/reasoning-inductives.html#coq:tacn.cofix
-    for a clarification on the [cofix] tactic.
+(**
+  Congratulations on reaching the end of this short tutorial - I don't have
+  enough time for more explanations... in case of doubt, refer to
+  https://coq.inria.fr/refman/language/core/coinductive.html
+  to read a bit more about coinduction and to
+  https://coq.inria.fr/refman/proofs/writing-proofs/reasoning-inductives.html#coq:tacn.cofix
+  for a clarification on the [cofix] tactic.
 
-    To help you learn what coinductive types are, how to do proofs by coinduction
-    and how to define corecursive functions, I prepared a few exercises for you...
+  To help you learn what coinductive types are, how to do proofs by coinduction
+  and how to define corecursive functions, I prepared a few exercises for you...
 
-    Good luck!
+  Good luck!
 
-    But beware: some of the theorems may be false, and I don't remember which ones... *)
+  But beware: some of the theorems may be false, and I don't remember which ones...
+*)
 
 Lemma succ_pred :
   forall n m : conat,
@@ -180,7 +196,8 @@ Proof.
 Admitted.
 
 Lemma sim_succ_omega :
-  forall n : conat, sim n (succ n) -> sim n omega.
+  forall n : conat,
+    sim n (succ n) -> sim n omega.
 Proof.
 Admitted.
 
@@ -190,28 +207,34 @@ Proof.
 Admitted.
 
 Lemma sim_succ :
-  forall n m : conat, sim n m -> sim (succ n) (succ m).
+  forall n m : conat,
+    sim n m -> sim (succ n) (succ m).
 Proof.
 Admitted.
 
 Lemma sim_succ_inv :
-  forall n m : conat, sim (succ n) (succ m) -> sim n m.
+  forall n m : conat,
+    sim (succ n) (succ m) -> sim n m.
 Proof.
 Admitted.
 
 (** ** Addition *)
 
-(** Define addition of conatural numbers and prove its properties. *)
+(**
+  Define addition of conatural numbers and prove its properties.
+*)
 
 Axiom add : conat -> conat -> conat.
 
 Lemma add_zero_l :
-  forall n m : conat, pred n = None -> add n m = m.
+  forall n m : conat,
+    pred n = None -> add n m = m.
 Proof.
 Admitted.
 
 Lemma add_zero_r :
-  forall n : conat, sim (add n zero) n.
+  forall n : conat,
+    sim (add n zero) n.
 Proof.
 Admitted.
 
@@ -222,32 +245,38 @@ Proof.
 Admitted.
 
 Lemma add_omega_l :
-  forall n : conat, sim (add omega n) omega.
+  forall n : conat,
+    sim (add omega n) omega.
 Proof.
 Admitted.
 
 Lemma add_omega_r :
-  forall n : conat, sim (add n omega) omega.
+  forall n : conat,
+    sim (add n omega) omega.
 Proof.
 Admitted.
 
 Lemma add_succ_l :
-  forall n m : conat, add (succ n) m = succ (add n m).
+  forall n m : conat,
+    add (succ n) m = succ (add n m).
 Proof.
 Admitted.
 
 Lemma add_succ_r :
-  forall n m : conat, sim (add n (succ m)) (succ (add n m)).
+  forall n m : conat,
+    sim (add n (succ m)) (succ (add n m)).
 Proof.
 Admitted.
 
 Lemma eq_sim :
-  forall n m : conat, n = m -> sim n m.
+  forall n m : conat,
+    n = m -> sim n m.
 Proof.
 Admitted.
 
 Lemma add_assoc :
-  forall a b c : conat, sim (add (add a b) c) (add a (add b c)).
+  forall a b c : conat,
+    sim (add (add a b) c) (add a (add b c)).
 Proof.
 Admitted.
 
@@ -258,7 +287,8 @@ Proof.
 Admitted.
 
 Lemma add_comm :
-  forall n m : conat, sim (add n m) (add m n).
+  forall n m : conat,
+    sim (add n m) (add m n).
 Proof.
 Admitted.
 
@@ -288,22 +318,27 @@ Admitted.
 
 (** ** Ordering *)
 
-(** Define the ordering (named [le]) on conatural numbers and prove its properties. *)
+(**
+  Define the ordering (named [le]) on conatural numbers and prove its properties.
+*)
 
 Axiom le : conat -> conat -> Prop.
 
 Lemma le_0_l :
-  forall n : conat, le zero n.
+  forall n : conat,
+    le zero n.
 Proof.
 Admitted.
 
 Lemma le_0_r :
-  forall n : conat, le n zero -> n = zero.
+  forall n : conat,
+    le n zero -> n = zero.
 Proof.
 Admitted.
 
 Lemma le_succ :
-  forall n m : conat, le n m -> le (succ n) (succ m).
+  forall n m : conat,
+    le n m -> le (succ n) (succ m).
 Proof.
 Admitted.
 
@@ -314,12 +349,14 @@ Proof.
 Admitted.
 
 Lemma le_refl :
-  forall n : conat, le n n.
+  forall n : conat,
+    le n n.
 Proof.
 Admitted.
 
 Lemma le_trans :
-  forall a b c : conat, le a b -> le b c -> le a c.
+  forall a b c : conat,
+    le a b -> le b c -> le a c.
 Proof.
 Admitted.
 
@@ -336,17 +373,20 @@ Proof.
 Admitted.
 
 Lemma le_omega_r :
-  forall n : conat, le n omega.
+  forall n : conat,
+    le n omega.
 Proof.
 Admitted.
 
 Lemma le_omega_l :
-  forall n : conat, le omega n -> sim n omega.
+  forall n : conat,
+    le omega n -> sim n omega.
 Proof.
 Admitted.
 
 Lemma le_succ_r :
-  forall n m : conat, le n m -> le n (succ m).
+  forall n m : conat,
+    le n m -> le n (succ m).
 Proof.
 Admitted.
 
@@ -369,12 +409,14 @@ Proof.
 Admitted.
 
 Lemma le_add_l' :
-  forall n m : conat, le n (add n m).
+  forall n m : conat,
+    le n (add n m).
 Proof.
 Admitted.
 
 Lemma le_add_r' :
-  forall n m : conat, le m (add n m).
+  forall n m : conat,
+    le m (add n m).
 Proof.
 Admitted.
 
@@ -392,27 +434,33 @@ Admitted.
 
 (** ** Min and max *)
 
-(** Define the functions [min] and [max] and prove their properties. *)
+(**
+  Define the functions [min] and [max] and prove their properties.
+*)
 
 Axiom min max : conat -> conat -> conat.
 
 Lemma min_zero_l :
-  forall n : conat, min zero n = zero.
+  forall n : conat,
+    min zero n = zero.
 Proof.
 Admitted.
 
 Lemma min_zero_r :
-  forall n : conat, min n zero = zero.
+  forall n : conat,
+    min n zero = zero.
 Proof.
 Admitted.
 
 Lemma min_omega_l :
-  forall n : conat, sim (min omega n) n.
+  forall n : conat,
+    sim (min omega n) n.
 Proof.
 Admitted.
 
 Lemma min_omega_r :
-  forall n : conat, sim (min n omega) n.
+  forall n : conat,
+    sim (min n omega) n.
 Proof.
 Admitted.
 
@@ -423,22 +471,26 @@ Proof.
 Admitted.
 
 Lemma max_zero_l :
-  forall n : conat, sim (max zero n) n.
+  forall n : conat,
+    sim (max zero n) n.
 Proof.
 Admitted.
 
 Lemma max_zero_r :
-  forall n : conat, sim (max n zero) n.
+  forall n : conat,
+    sim (max n zero) n.
 Proof.
 Admitted.
 
 Lemma max_omega_l :
-  forall n : conat, sim (max omega n) omega.
+  forall n : conat,
+    sim (max omega n) omega.
 Proof.
 Admitted.
 
 Lemma max_omega_r :
-  forall n : conat, sim (max n omega) omega.
+  forall n : conat,
+    sim (max n omega) omega.
 Proof.
 Admitted.
 
@@ -449,42 +501,50 @@ Proof.
 Admitted.
 
 Lemma min_assoc :
-  forall a b c : conat, sim (min (min a b) c) (min a (min b c)).
+  forall a b c : conat,
+    sim (min (min a b) c) (min a (min b c)).
 Proof.
 Admitted.
 
 Lemma max_assoc :
-  forall a b c : conat, sim (max (max a b) c) (max a (max b c)).
+  forall a b c : conat,
+    sim (max (max a b) c) (max a (max b c)).
 Proof.
 Admitted.
 
 Lemma min_comm :
-  forall n m : conat, sim (min n m) (min m n).
+  forall n m : conat,
+    sim (min n m) (min m n).
 Proof.
 Admitted.
 
 Lemma max_comm :
-  forall n m : conat, sim (max n m) (max m n).
+  forall n m : conat,
+    sim (max n m) (max m n).
 Proof.
 Admitted.
 
 Lemma min_le :
-  forall n m : conat, le n m -> sim (min n m) n.
+  forall n m : conat,
+    le n m -> sim (min n m) n.
 Proof.
 Admitted.
 
 Lemma max_le :
-  forall n m : conat, le n m -> sim (max n m) m.
+  forall n m : conat,
+    le n m -> sim (max n m) m.
 Proof.
 Admitted.
 
 Lemma min_diag :
-  forall n : conat, sim (min n n) n.
+  forall n : conat,
+    sim (min n n) n.
 Proof.
 Admitted.
 
 Lemma max_diag :
-  forall n : conat, sim (max n n) n.
+  forall n : conat,
+    sim (max n n) n.
 Proof.
 Admitted.
 
@@ -519,12 +579,14 @@ Proof.
 Admitted.
 
 Lemma min_max :
-  forall a b : conat, sim (min a (max a b)) a.
+  forall a b : conat,
+    sim (min a (max a b)) a.
 Proof.
 Admitted.
 
 Lemma max_min :
-  forall a b : conat, sim (max a (min a b)) a.
+  forall a b : conat,
+    sim (max a (min a b)) a.
 Proof.
 Admitted.
 
@@ -542,8 +604,10 @@ Admitted.
 
 (** ** Division by 2 *)
 
-(** Define the function [div2], which halves a conatural number, and prove its
-    properties. *)
+(**
+  Define the function [div2], which halves a conatural number, and prove its
+  properties.
+*)
 
 Axiom div2 : conat -> conat.
 
@@ -558,35 +622,44 @@ Proof.
 Admitted.
 
 Lemma div2_succ :
-  forall n : conat, sim (div2 (succ (succ n))) (succ (div2 n)).
+  forall n : conat,
+    sim (div2 (succ (succ n))) (succ (div2 n)).
 Proof.
 Admitted.
 
 Lemma div2_add :
-  forall n : conat, sim (div2 (add n n)) n.
+  forall n : conat,
+    sim (div2 (add n n)) n.
 Proof.
 Admitted.
 
 Lemma le_div2_l' :
-  forall n m : conat, le n m -> le (div2 n) m.
+  forall n m : conat,
+    le n m -> le (div2 n) m.
 Proof.
 Admitted.
 
 Lemma le_div2_l :
-  forall n : conat, le (div2 n) n.
+  forall n : conat,
+    le (div2 n) n.
 Proof.
 Admitted.
 
 Lemma le_div2 :
-  forall n m : conat, le n m -> le (div2 n) (div2 m).
+  forall n m : conat,
+    le n m -> le (div2 n) (div2 m).
 Proof.
 Admitted.
 
 (** ** [Finite] and [Infinite] *)
 
-(** Define the predicates [Finite] and [Infinite]. Prove the lemmas below. *)
+(**
+  Define the predicates [Finite] and [Infinite]. Prove the lemmas below.
+*)
 
-Axiom Finite Infinite : conat -> Prop.
+Axioms
+  (Finite : conat -> Prop)
+  (Infinite : conat -> Prop).
 
 Lemma omega_not_Finite :
   ~ Finite omega.
@@ -599,17 +672,20 @@ Proof.
 Admitted.
 
 Lemma Infinite_omega' :
-  forall n : conat, Infinite n -> sim n omega.
+  forall n : conat,
+    Infinite n -> sim n omega.
 Proof.
 Admitted.
 
 Lemma Finite_Infinite :
-  forall n : conat, Finite n -> Infinite n -> False.
+  forall n : conat,
+    Finite n -> Infinite n -> False.
 Proof.
 Admitted.
 
 Lemma Finite_or_Infinite :
-  forall c : conat, ~ ~ (Finite c \/ Infinite c).
+  forall c : conat,
+    ~ ~ (Finite c \/ Infinite c).
 Proof.
 Admitted.
 
@@ -639,10 +715,14 @@ Admitted.
 
 (** ** [Even] and [Odd] *)
 
-(** Define the predicates [Even] and [Odd]. Prove the lemmas below. Bonus points
-    if you use mutual coinductive types for the definition. *)
+(**
+  Define the predicates [Even] and [Odd]. Prove the lemmas below. Bonus points
+  if you use mutual coinductive types for the definition.
+*)
 
-Axiom Even Odd : conat -> Prop.
+Axioms
+  (Even : conat -> Prop)
+  (Odd : conat -> Prop).
 
 Lemma Even_zero :
   Even zero.
@@ -665,69 +745,84 @@ Proof.
 Admitted.
 
 Lemma Even_Odd_Infinite :
-  forall n : conat, Even n -> Odd n -> Infinite n.
+  forall n : conat,
+    Even n -> Odd n -> Infinite n.
 Proof.
 Admitted.
 
 Lemma Even_succ :
-  forall n : conat, Odd n -> Even (succ n).
+  forall n : conat,
+    Odd n -> Even (succ n).
 Proof.
 Admitted.
 
 Lemma Odd_succ :
-  forall n : conat, Even n -> Odd (succ n).
+  forall n : conat,
+    Even n -> Odd (succ n).
 Proof.
 Admitted.
 
 Lemma Even_succ_inv :
-  forall n : conat, Odd (succ n) -> Even n.
+  forall n : conat,
+    Odd (succ n) -> Even n.
 Proof.
 Admitted.
 
 Lemma Odd_succ_inv :
-  forall n : conat, Even (succ n) -> Odd n.
+  forall n : conat,
+    Even (succ n) -> Odd n.
 Proof.
 Admitted.
 
 Lemma Finite_Even_Odd :
-  forall n : conat, Finite n -> Even n \/ Odd n.
+  forall n : conat,
+    Finite n -> Even n \/ Odd n.
 Proof.
 Admitted.
 
 Lemma Finite_not_both_Even_Odd :
-  forall n : conat, Finite n -> ~ (Even n /\ Odd n).
+  forall n : conat,
+    Finite n -> ~ (Even n /\ Odd n).
 Proof.
 Admitted.
 
 Lemma Even_add_Odd :
-  forall n m : conat, Odd n -> Odd m -> Even (add n m).
+  forall n m : conat,
+    Odd n -> Odd m -> Even (add n m).
 Proof.
 Admitted.
 
 Lemma Even_add_Even :
-  forall n m : conat, Even n -> Even m -> Even (add n m).
+  forall n m : conat,
+    Even n -> Even m -> Even (add n m).
 Proof.
 Admitted.
 
 Lemma Odd_add :
-  forall n m : conat, Even n -> Odd m -> Odd (add n m).
+  forall n m : conat,
+    Even n -> Odd m -> Odd (add n m).
 Proof.
 Admitted.
 
 (** ** Multiplication *)
 
-(** Define multiplication of conatural numbers. Formulate and prove its properties
-    (hint: they are very similar to properties of natural number multiplication). *)
+(**
+  Define multiplication of conatural numbers. Formulate and prove its properties
+  (hint: they are very similar to properties of natural number multiplication).
+*)
 
 (** ** Naturals and conaturals *)
 
-(** Define the function [from_nat] which transforms a natural number into its
-    corresponding conatural number. *)
+(**
+  Define the function [from_nat] which transforms a natural number into its
+  corresponding conatural number.
+*)
 
 Axiom from_nat : nat -> conat.
 
 Lemma Finite_from_nat :
-  forall n : nat, Finite (from_nat n).
+  forall n : nat,
+    Finite (from_nat n).
 Proof.
 Admitted.
 
