src/Duality.v
@@ -1,32 +1,32 @@
 Module ind.
 
 Inductive nat : Type :=
-    | Z : nat
-    | S : nat -> nat.
+| Z : nat
+| S : nat -> nat.
 
 Inductive list (A : Type) : Type :=
-    | nil : list A
-    | cons : A -> list A -> list A.
+| nil : list A
+| cons : A -> list A -> list A.
 
 Arguments nil {A}.
 Arguments cons {A} _ _.
 
 Fixpoint len {A : Type} (l : list A) {struct l} : nat :=
 match l with
-    | nil => Z
-    | cons _ t => S (len t)
+| nil => Z
+| cons _ t => S (len t)
 end.
 
 Definition pred (n : nat) : option nat :=
 match n with
-    | Z => None
-    | S n' => Some n'
+| Z => None
+| S n' => Some n'
 end.
 
 Definition uncons {A : Type} (l : list A) : option (A * list A) :=
 match l with
-    | nil => None
-    | cons h t => Some (h, t)
+| nil => None
+| cons h t => Some (h, t)
 end.
 
 End ind.
@@ -35,43 +35,43 @@ Module coind.
 
 CoInductive conat : Type :=
 {
-    pred : option conat;
+  pred : option conat;
 }.
 
 CoInductive colist (A : Type) : Type :=
 {
-    uncons : option (A * colist A);
+  uncons : option (A * colist A);
 }.
 
 Arguments uncons {A}.
 
 CoFixpoint colen {A : Type} (l : colist A) : conat :=
 {|
-    pred :=
-      match uncons l with
-          | None => None
-          | Some (_, t) => Some (colen t)
-      end
+  pred :=
+    match uncons l with
+        | None => None
+        | Some (_, t) => Some (colen t)
+    end
 |}.
 
 Definition Z : conat :=
 {|
-    pred := None
+  pred := None
 |}.
 
 Definition S (c : conat) : conat :=
 {|
-    pred := Some c
+  pred := Some c
 |}.
 
 Definition nil {A : Type} : colist A :=
 {|
-    uncons := None
+  uncons := None
 |}.
 
 Definition cons {A : Type} (h : A) (t : colist A) : colist A :=
 {|
-    uncons := Some (h, t)
+  uncons := Some (h, t)
 |}.
 
 End coind.
